update

testcase/ProofRTT/SecurityProof.v
@@ -24,7 +24,45 @@ Definition SecState := ZMap.t SecureRealmState.
 (************************************************************************************)
 
 Parameter addr_to_gidx: Z -> Z.
-Parameter walk_rtt: Shared -> Z -> Z -> option Z.
+Parameter gfn_to_rtt_offs: Z -> Z -> Z.
+Parameter gfn_to_pte_offs: Z -> Z -> Z.
+Parameter ADDR_MASK: Z.
+Parameter PTE_VALID: Z.
+
+Definition walk_one_step sh lvl gfn rtt_idx :=
+  let offs := gfn_to_rtt_offs gfn lvl in
+  let pte := (sh.(granule_data) @ rtt_idx).(g_norm) @ offs in
+  let addr := pte & ADDR_MASK in
+  let gidx := addr_to_gidx addr in
+  (gidx, pte).
+
+Fixpoint walk_rtt_level (n: nat) (sh: Shared) (lvl: Z) (rd: Z) (gfn: Z) (rtt_idx: Z) (pte: Z) :=
+  match n with
+  | O => (lvl, rtt_idx, pte)
+  | S n' =>
+    match walk_rtt_level n' sh lvl rd gfn rtt_idx pte with
+    | (lvl', rtt_idx', pte') =>
+      if ((pte & PTE_VALID) =? PTE_VALID) && ((sh.(granules) @ rtt_idx').(e_state) =? GRANULE_STATE_RTT) then
+        let (gidx, pte') := walk_one_step sh lvl' gfn rtt_idx' in
+        (lvl' + 1, gidx, pte')
+      else
+        (lvl', rtt_idx', pte')
+    end
+  end.
+
+Definition rd_rtt sh rd := (sh.(granule_data) @ rd).(g_rd).(e_rd_s2_ctx).(e_rls2ctx_g_rtt).
+
+Definition walk_rtt sh rd gfn :=
+  let rtt_idx := rd_rtt sh rd in
+  match walk_rtt_level 4%nat sh 0 rd gfn rtt_idx 0 with
+  | (lvl', idx', pte') =>
+    if (pte' & PTE_VALID) <>? PTE_VALID then None
+    else Some (idx' + gfn_to_pte_offs lvl' gfn)
+  end.
+
+Lemma walk_rtt_same_set_slot:
+  forall sh sl rd ipa, walk_rtt (sh.[slots] :< sl) rd ipa = walk_rtt sh rd ipa.
+Admitted.
 
 Lemma walk_rtt_same:
   forall sh' sh rd ipa,
@@ -319,6 +357,155 @@ Ltac ext_repl Rsec Rnorm :=
 
 Ltac Frewrite := repeat (repeat rewrite_id; frewrite).
 
+
+Lemma smc_rtt_fold_3_inv:
+  forall s2_ctx map_addr wi call15 call34 call44 call33 norm_d_init norm_d ret_n norm_d'
+    (Hspec: smc_rtt_fold_3 s2_ctx map_addr wi call15 call34 call44 call33 norm_d_init norm_d = Some (ret_n, norm_d'))
+    (Hinv: SharedInv norm_d.(share)),
+    SharedInv norm_d'.(share).
+Admitted.
+
+Lemma granule_data_slots_update_permu:
+  forall st v0 v1, ((share st).[granule_data] :< v0).[slots] :< v1 = ((share st).[slots] :< v1).[granule_data] :< v0.
+Proof. easy. Qed.
+
+Definition smc_rtt_fold_3 (v_s2_ctx: Ptr) (v_map_addr: Z) (v_wi: Ptr) (v_call15: Ptr) (v_call34: Ptr) (v_call44: Z) (v_call33: Ptr) (st_0: RData) (st_34: RData) : (option (Z * RData)) :=
+  rely (((v_s2_ctx.(pbase)) = ("stack_s2_ctx")));
+  rely (((v_s2_ctx.(poffset)) = (0)));
+  rely (((v_wi.(pbase)) = ("stack_wi")));
+  rely (((v_wi.(poffset)) = (0)));
+  rely (((v_call15.(pbase)) = ("slot_rtt")));
+  rely (((v_call34.(pbase)) = ("slot_rtt2")));
+  rely (((v_call33.(pbase)) = ("granules")));
+  rely ((((st_34.(share)).(granules)) @ (((st_34.(share)).(slots)) @ SLOT_RTT)).(e_state) = GRANULE_STATE_RTT);
+  rely ((((st_34.(share)).(granules)) @ (((st_34.(share)).(slots)) @ SLOT_RTT2)).(e_state) = GRANULE_STATE_RTT);
+  when cid == (((((st_34.(share)).(granules)) @ (((st_34.(share)).(slots)) @ SLOT_RTT)).(e_lock)));
+  when cid_0 == (((((st_34.(share)).(granules)) @ (((st_34.(share)).(slots)) @ SLOT_RTT2)).(e_lock)));
+  rely ((((v_call33.(pbase)) = ("granules")) /\ ((((v_call33.(poffset)) mod (ST_GRANULE_SIZE)) = (0)))));
+  rely ((((st_34.(share)).(slots)) @ SLOT_RTT) <> (((st_34.(share)).(slots)) @ SLOT_RTT2)); (* MANUALLY ADDED *)
+  if (
+    match (((((st_34.(share)).(granules)) @ (((v_call33.(poffset)) + (4)) / (ST_GRANULE_SIZE))).(e_lock))) with
+    | (Some cid_1) => true
+    | None => false
+    end)
+  then (
+    when cid_1 == (((((st_34.(share)).(granules)) @ (((v_call33.(poffset)) + (4)) / (ST_GRANULE_SIZE))).(e_lock)));
+    rely (((v_call34.(poffset)) = (0)));
+    rely ((((0 - (CPU_ID)) <= (0)) /\ ((CPU_ID < (16)))));
+    rely (((v_call15.(poffset)) = (0)));
+    rely (((((((st_34.(stack)).(stack_wi)).(e_g_llt)) - (STACK_VIRT)) < (0)) /\ ((((((st_34.(stack)).(stack_wi)).(e_g_llt)) - (GRANULES_BASE)) >= (0)))));
+    rely ((((st_34.(share)).(slots)) @ SLOT_RTT) = ((st_34.(stack)).(stack_wi)).(e_g_llt)); (* MANUALLY ADDED *)
+    rely (exists rd gfn lvl pte pte',  (* MANUALLY ADDED *)
+          ((st_34.(share).(granules) @ rd).(e_state) = GRANULE_STATE_RD)
+          /\ walk_rtt_level (Z.to_nat lvl) (st_34.(share)) 0 rd gfn (rd_rtt (st_34.(share)) rd) 0 =
+              (lvl, (((st_34.(stack)).(stack_wi)).(e_g_llt)), pte)
+          /\ gfn_to_rtt_offs gfn lvl = 8 * (((st_34.(stack)).(stack_wi)).(e_index))
+          /\ walk_one_step (st_34.(share)) lvl gfn (((st_34.(stack)).(stack_wi)).(e_g_llt)) = ((((st_34.(share)).(slots)) @ SLOT_RTT2), pte'));
+    (Some (
+      0  ,
+      (((lens 106 st_34).[share].[granule_data] :<
+        ((((st_34.(share)).(granule_data)) #
+          (((st_34.(share)).(slots)) @ SLOT_RTT) ==
+          ((((st_34.(share)).(granule_data)) @ (((st_34.(share)).(slots)) @ SLOT_RTT)).[g_norm] :<
+            (((((st_34.(share)).(granule_data)) @ (((st_34.(share)).(slots)) @ SLOT_RTT)).(g_norm)) #
+              ((v_call15.(poffset)) + ((8 * ((((st_34.(stack)).(stack_wi)).(e_index)))))) ==
+              v_call44))) #
+          (((st_34.(share)).(slots)) @ SLOT_RTT2) ==
+          (((((st_34.(share)).(granule_data)) #
+            (((st_34.(share)).(slots)) @ SLOT_RTT) ==
+            ((((st_34.(share)).(granule_data)) @ (((st_34.(share)).(slots)) @ SLOT_RTT)).[g_norm] :<
+              (((((st_34.(share)).(granule_data)) @ (((st_34.(share)).(slots)) @ SLOT_RTT)).(g_norm)) #
+                ((v_call15.(poffset)) + ((8 * ((((st_34.(stack)).(stack_wi)).(e_index)))))) ==
+                v_call44))) @ (((st_34.(share)).(slots)) @ SLOT_RTT2)).[g_norm] :<
+            zero_granule_data_normal))).[share].[slots] :<
+        ((((st_34.(share)).(slots)) # SLOT_RTT2 == (- 1)) # SLOT_RTT == (- 1)))
+    )))
+  else None.
+
+Record lens_field_same: Prop := {
+    lens_gpt_same: forall st v, gpt (share (lens v st)) = gpt (share st)
+  }.
+
+Parameter lens_field_same_prop: lens_field_same.
+
+Ltac rewrite_lens :=
+  match goal with
+  | [|- context[gpt (share (lens ?v ?st))] ] => rewrite (lens_gpt_same lens_field_same_prop st v)
+  | [H: context[gpt (share (lens ?v ?st)) ] |- _] => rewrite (lens_gpt_same lens_field_same_prop st v) in H
+  end.
+
+Lemma smc_rtt_fold_3_secure:
+  forall sec_d sec_st norm_d (Hrel: relate sec_d sec_st norm_d)
+    s2_ctx map_addr wi call15 call34 call44 call33 norm_d_init ret_n ret_s sec_d' norm_d'
+    (Hnorm: smc_rtt_fold_3 s2_ctx map_addr wi call15 call34 call44 call33 norm_d_init norm_d = Some (ret_n, norm_d'))
+    (Hsec: smc_rtt_fold_3 s2_ctx map_addr wi call15 call34 call44 call33 norm_d_init sec_d = Some (ret_s, sec_d'))
+    (Hinv: SharedInv (norm_d.(share))),
+    ret_s = ret_n /\ relate sec_d' sec_st norm_d'.
+Proof.
+  intros. pose proof Hrel as D. destruct D.
+  unfold smc_rtt_fold_3 in *; autounfold with sem in *.
+  repeat simpl_hyp Hsec. repeat simpl_hyp Hnorm. inv Hnorm.
+  destruct e11 as (? & ? & ? & ? & ? & ? & ? & ? & ?).
+  clear C19.
+  Frewrite. simpl_hyp Hsec. inv Hsec.
+  extract_prop.
+  split.
+  - reflexivity.
+  - constructor.
+    {
+      constructor; simpl.
+      inv relate_sec_data0.
+      rewrite_id.
+      remember ((e_g_llt (stack_wi (stack norm_d)))) as rtt_idx. symmetry in Heqrtt_idx.
+      remember ((slots (share sec_d)) @ SLOT_RTT2) as rtt2_idx. symmetry in Heqrtt2_idx.
+      remember (match e_index (stack_wi (stack norm_d)) with | 0 => 0  | Z.pos y' => Z.pos y'~0~0~0 | Z.neg y' => Z.neg y'~0~0~0 end) as e_idx.
+      remember (poffset call15) as call15_ofs. symmetry in Heqcall15_ofs.
+      remember (call15_ofs + e_idx) as g_norm_idx. symmetry in Heqg_norm_idx.
+      remember ((granule_data (share sec_d))) as granule_data_sec. symmetry in Heqgranule_data_sec.
+      intros.
+      rewrite lens_same in Hrd. repeat rewrite_id.
+      repeat rewrite lens_same in Hwalk.
+      match type of Hwalk with
+      | walk_rtt ?d ?rd ?addr = _ =>
+        assert(Hwalk_eq: walk_rtt d rd addr = walk_rtt (share sec_d) rd addr)
+      end.
+      {
+        rewrite Heqrtt2_idx.
+        assert_gso. lia. rewrite (ZMap.gso _ _ Hneq).
+        rewrite walk_rtt_same_set_slot.
+
+        admit.
+      }
+      rewrite Hwalk_eq in Hwalk.
+      pose proof (mem_rel0 rd_gidx Hrd vaddr data_gidx Hwalk) as mem_rel.
+      simpl in mem_rel.
+      inv Hinv. unfold rtt_map_data in *.
+      erewrite relate_walk_rtt_same in *; try eassumption.
+      pose proof (rtt_map_data_inv0 rd_gidx Hrd (addr_to_gidx vaddr) data_gidx Hwalk) as Hdata.
+      autounfold with spec in *.
+      assert_gso. red; intro T; inv T; lia.
+      rewrite (ZMap.gso _ _ Hneq).
+      assert_gso. red; intro T; inv T; lia.
+      rewrite (ZMap.gso _ _ Hneq0).
+      rewrite (ZMap.gso _ _ Hneq).
+      rewrite (ZMap.gso _ _ Hneq0).
+      assumption.
+    }
+    {
+      pose proof relate_share0 as D; destruct D.
+      constructor; simpl; repeat rewrite lens_same; rewrite_id; try reflexivity.
+      all:intros; rewrite_id; simpl; repeat (destruct_zmap; simpl; rewrite_id); try reflexivity.
+      all:rewrite id_g_norm0; rewrite_id; subst; try reflexivity; try assumption.
+    }
+    {
+      constructor; simpl; repeat rewrite lens_same; rewrite_id; try reflexivity.
+    }
+Qed.
+
+
+
+
+
 Lemma realm_access_mem_inv:
   forall rd addr val nd nd' ret_d
     (Hspec: normal_realm_access_mem rd addr val nd = Some (nd', ret_d))
@@ -465,169 +652,12 @@ Proof.
     split. reflexivity. assumption.
 Qed.
 
-Lemma smc_rtt_fold_3_inv:
-  forall s2_ctx map_addr wi call15 call34 call44 call33 norm_d_init norm_d ret_n norm_d'
-    (Hspec: smc_rtt_fold_3 s2_ctx map_addr wi call15 call34 call44 call33 norm_d_init norm_d = Some (ret_n, norm_d'))
-    (Hinv: SharedInv norm_d.(share)),
-    SharedInv norm_d'.(share).
-Admitted.
 
-Lemma granule_data_slots_update_permu:
-  forall st v0 v1, ((share st).[granule_data] :< v0).[slots] :< v1 = ((share st).[slots] :< v1).[granule_data] :< v0.
-Proof. easy. Qed.
-
-Definition smc_rtt_fold_3 (v_s2_ctx: Ptr) (v_map_addr: Z) (v_wi: Ptr) (v_call15: Ptr) (v_call34: Ptr) (v_call44: Z) (v_call33: Ptr) (st_0: RData) (st_34: RData) : (option (Z * RData)) :=
-  rely (((v_s2_ctx.(pbase)) = ("stack_s2_ctx")));
-  rely (((v_s2_ctx.(poffset)) = (0)));
-  rely (((v_wi.(pbase)) = ("stack_wi")));
-  rely (((v_wi.(poffset)) = (0)));
-  rely (((v_call15.(pbase)) = ("slot_rtt")));
-  rely (((v_call34.(pbase)) = ("slot_rtt2")));
-  rely (((v_call33.(pbase)) = ("granules")));
-  rely ((((st_34.(share)).(granules)) @ (((st_34.(share)).(slots)) @ SLOT_RTT)).(e_state) = GRANULE_STATE_RTT);
-  rely ((((st_34.(share)).(granules)) @ (((st_34.(share)).(slots)) @ SLOT_RTT2)).(e_state) = GRANULE_STATE_RTT);
-  when cid == (((((st_34.(share)).(granules)) @ (((st_34.(share)).(slots)) @ SLOT_RTT)).(e_lock)));
-  when cid_0 == (((((st_34.(share)).(granules)) @ (((st_34.(share)).(slots)) @ SLOT_RTT2)).(e_lock)));
-  rely ((((v_call33.(pbase)) = ("granules")) /\ ((((v_call33.(poffset)) mod (ST_GRANULE_SIZE)) = (0)))));
-  if (
-    match (((((st_34.(share)).(granules)) @ (((v_call33.(poffset)) + (4)) / (ST_GRANULE_SIZE))).(e_lock))) with
-    | (Some cid_1) => true
-    | None => false
-    end)
-  then (
-    when cid_1 == (((((st_34.(share)).(granules)) @ (((v_call33.(poffset)) + (4)) / (ST_GRANULE_SIZE))).(e_lock)));
-    rely (((v_call34.(poffset)) = (0)));
-    rely ((((0 - (CPU_ID)) <= (0)) /\ ((CPU_ID < (16)))));
-    rely (((v_call15.(poffset)) = (0)));
-    rely (((((((st_34.(stack)).(stack_wi)).(e_g_llt)) - (STACK_VIRT)) < (0)) /\ ((((((st_34.(stack)).(stack_wi)).(e_g_llt)) - (GRANULES_BASE)) >= (0)))));
-    (Some (
-      0  ,
-      (((lens 106 st_34).[share].[granule_data] :<
-        ((((st_34.(share)).(granule_data)) #
-          (((st_34.(share)).(slots)) @ SLOT_RTT) ==
-          ((((st_34.(share)).(granule_data)) @ (((st_34.(share)).(slots)) @ SLOT_RTT)).[g_norm] :<
-            (((((st_34.(share)).(granule_data)) @ (((st_34.(share)).(slots)) @ SLOT_RTT)).(g_norm)) #
-              ((v_call15.(poffset)) + ((8 * ((((st_34.(stack)).(stack_wi)).(e_index)))))) ==
-              v_call44))) #
-          (((st_34.(share)).(slots)) @ SLOT_RTT2) ==
-          (((((st_34.(share)).(granule_data)) #
-            (((st_34.(share)).(slots)) @ SLOT_RTT) ==
-            ((((st_34.(share)).(granule_data)) @ (((st_34.(share)).(slots)) @ SLOT_RTT)).[g_norm] :<
-              (((((st_34.(share)).(granule_data)) @ (((st_34.(share)).(slots)) @ SLOT_RTT)).(g_norm)) #
-                ((v_call15.(poffset)) + ((8 * ((((st_34.(stack)).(stack_wi)).(e_index)))))) ==
-                v_call44))) @ (((st_34.(share)).(slots)) @ SLOT_RTT2)).[g_norm] :<
-            zero_granule_data_normal))).[share].[slots] :<
-        ((((st_34.(share)).(slots)) # SLOT_RTT2 == (- 1)) # SLOT_RTT == (- 1)))
-    )))
-  else None.
-
-Record lens_field_same: Prop := {
-    lens_gpt_same: forall st v, gpt (share (lens v st)) = gpt (share st)
-  }.
-
-Parameter lens_field_same_prop: lens_field_same.
-
-Ltac rewrite_lens :=
-  match goal with
-  | [|- context[gpt (share (lens ?v ?st))] ] => rewrite (lens_gpt_same lens_field_same_prop st v)
-  | [H: context[gpt (share (lens ?v ?st)) ] |- _] => rewrite (lens_gpt_same lens_field_same_prop st v) in H
-  end.
-
-Lemma smc_rtt_fold_3_secure:
-  forall sec_d sec_st norm_d (Hrel: relate sec_d sec_st norm_d)
-    s2_ctx map_addr wi call15 call34 call44 call33 norm_d_init ret_n ret_s sec_d' norm_d'
-    (Hnorm: smc_rtt_fold_3 s2_ctx map_addr wi call15 call34 call44 call33 norm_d_init norm_d = Some (ret_n, norm_d'))
-    (Hsec: smc_rtt_fold_3 s2_ctx map_addr wi call15 call34 call44 call33 norm_d_init sec_d = Some (ret_s, sec_d'))
-    (Hinv: SharedInv (norm_d.(share))),
-    ret_s = ret_n /\ relate sec_d' sec_st norm_d'.
-Proof.
-  intros. pose proof Hrel as D. destruct D.
-  unfold smc_rtt_fold_3 in *; autounfold with sem in *.
-  repeat simpl_hyp Hsec; inv Hsec.
-  Frewrite. simpl_hyp Hnorm. inv Hnorm.
-  extract_prop.
-  split.
-  - reflexivity.
-  - constructor.
-    {
-      constructor; simpl.
-      inv relate_sec_data0.
-      rewrite_id.
-      remember ((slots (share sec_d)) @ SLOT_RTT) as rtt_idx.
-      remember ((slots (share sec_d)) @ SLOT_RTT2) as rtt2_idx.
-      remember ((g_norm (granule_data (share sec_d)) @ rtt_idx)).
-      remember (match e_index (stack_wi (stack norm_d)) with | 0 => 0  | Z.pos y' => Z.pos y'~0~0~0 | Z.neg y' => Z.neg y'~0~0~0 end) as e_idx.
-      remember (poffset call15) as call15_ofs.
-      remember (call15_ofs + e_idx) as g_norm_idx.
-      remember ((granule_data (share sec_d))) as granule_data_sec.
-      intros.
-      rewrite lens_same in Hrd. repeat rewrite_id.
-      repeat rewrite lens_same in Hwalk.
-      match type of Hwalk with
-      | walk_rtt ?d ?rd ?addr = _ =>
-        assert(Hwalk_eq: walk_rtt d rd addr = walk_rtt (share sec_d) rd addr)
-      end.
-      {
-        (*
-          need rely/prove
-          - rd_gidx is a valid RD
-          - walk_rtt_level (share sec_d) rd_gidx (addr_to_gidx map_addr) (level - 1) = Some (slots (share norm_d)) @ SLOT_RTT)
-            walk_rtt_level (share sec_d) rd_gidx (addr_to_gidx map_addr) level = Some (slots (share norm_d)) @ SLOT_RTT2)
-          - refcount == 0
-          - forall 0 <= i < 512, SLOT_RTT @ i = DESTROYED
-          - forall level, walk_rtt_level d rd addr level = Some pte -> pte = DESTROYED -> walk_rtt d rd addr = None
-          - 
-
-         *)
-        admit.
-      }
-      rewrite Hwalk_eq in Hwalk.
-      pose proof (mem_rel0 rd_gidx Hrd vaddr data_gidx Hwalk) as mem_rel.
-      simpl in mem_rel.
-      inv Hinv. unfold rtt_map_data in *.
-      erewrite relate_walk_rtt_same in *; try eassumption.
-      pose proof (rtt_map_data_inv0 rd_gidx Hrd (addr_to_gidx vaddr) data_gidx Hwalk) as Hdata.
-      autounfold with spec in *.
-      assert_gso. red; intro T; inv T; lia.
-      rewrite (ZMap.gso _ _ Hneq).
-      assert_gso. red; intro T; inv T; lia.
-      rewrite (ZMap.gso _ _ Hneq0).
-      rewrite (ZMap.gso _ _ Hneq).
-      rewrite (ZMap.gso _ _ Hneq0).
-      assumption.
-    }
-    {
-      pose proof relate_share0 as D; destruct D.
-      constructor; simpl; repeat rewrite lens_same; rewrite_id; try reflexivity.
-      all:intros; rewrite_id; simpl; repeat (destruct_zmap; simpl; rewrite_id); try reflexivity.
-      all:rewrite id_g_norm0; rewrite_id; subst; try reflexivity; try assumption.
-    }
-    {
-      constructor; simpl; repeat rewrite lens_same; rewrite_id; try reflexivity.
-    }
-Qed.
-
-constructor.
-intros.
-repeat simpl_hyp H0; inv H0.
-inv relate_sec_data0.
-
-  simpl in *.
-  rewrite e_state_lens_same in Hrd.
-  destruct Hinv.
-  unfold rtt_map_data in rtt_map_data_inv0.
-  simpl in Hwalk.
-
-  rewrite walk_rtt_slots_unrelated in Hwalk.
-  rewrite walk_rtt_granule_data_update_lens_same in Hwalk.
-
-
-
-  Lemma smc_granule_delegate_inv:
-  forall norm_d v_addr ret_n norm_d'
-    (Hspec: smc_granule_delegate_spec v_addr norm_d = Some (ret_n, norm_d'))
-    (Hinv: SharedInv norm_d.(share)),
-    SharedInv norm_d'.(share).
+Lemma smc_granule_delegate_inv:
+forall norm_d v_addr ret_n norm_d'
+  (Hspec: smc_granule_delegate_spec v_addr norm_d = Some (ret_n, norm_d'))
+  (Hinv: SharedInv norm_d.(share)),
+  SharedInv norm_d'.(share).
 (*
 
       - inv Hinv.
